chacha spec

code/salsa-family/Hacl.Impl.Chacha20.fst
@@ -502,7 +502,7 @@ val init:
 let init st k n =
   setup st k n 0ul;
   let h = ST.get() in
-  Ghost.elift2 (fun k n -> MkLog k n) (Ghost.hide (as_seq h k)) (Ghost.hide (as_seq h n))
+  Ghost.elift2 (fun (k:uint8_p{length k = 32 /\ live h k}) (n:uint8_p{length n = 12 /\ live h n}) -> MkLog (as_seq h k) (as_seq h n)) (Ghost.hide k) (Ghost.hide n)
 
 
 #reset-options "--initial_fuel 0 --max_fuel 0 --z3rlimit 100"
@@ -642,3 +642,26 @@ let rec chacha20_counter_mode output plain len log st ctr =
     let h = ST.get() in
     lemma_chacha20_counter_mode_2 h output h0 plain len h0 st (Ghost.reveal log).k (Ghost.reveal log).n ctr
   )
+
+#set-options "--lax"
+
+val chacha20:
+  output:uint8_p ->
+  plain:uint8_p{disjoint output plain} ->
+  len:U32.t{U32.v len = length output /\ U32.v len = length plain} ->
+  key:uint8_p{length key = 32} ->
+  nonce:uint8_p{length key = 12} ->
+  ctr:U32.t{U32.v ctr + (length plain / 64) < pow2 32} ->
+  Stack unit
+    (requires (fun h -> live h output /\ live h plain))
+    (ensures (fun h0 _ h1 -> live h1 output /\ live h0 plain
+      /\ modifies_1 output h0 h1))
+      (* /\ (let o = as_seq h1 output in *)
+      (*    let plain = as_seq h0 plain in *)
+      (*    o == Spec.CTR.counter_mode chacha20_ctx chacha20_cipher k n (U32.v ctr) plain))) *)
+let chacha20 output plain len k n ctr =
+  push_frame();
+  let st = alloc () in
+  let l  = init st k n in
+  let l' = chacha20_counter_mode output plain len l st ctr in
+  pop_frame()
